Make the push-pop stuff be more controlled

ind/DoublyLinkedListIface.fst
@@ -854,10 +854,8 @@ let auto_unchanged_node_connections_dll_valid h0 h1 d (n:node 'a) =
 /// you should ask someone who knows about how this library works to
 /// look at things.
 
-let auto_dll_valid_on_push h0 h1 d = ()
+let auto_dll_push_pop h0 h1 h2 h3 d = ()
 
-let auto_dll_fp_on_push h0 h1 d = ()
+let auto_dll_fp_push_pop h0 h1 h2 h3 d = ()
 
-let auto_dll_valid_on_pop h0 h1 d = _lemma_dll_valid_and_unchanged_through_pop h0 h1 d
-
-let auto_dll_fp_on_pop h0 h1 d = _lemma_dll_valid_and_unchanged_through_pop h0 h1 d
+let auto_dll_fp_disjoint_push h0 h1 d = ()
